Date: 26th January 2023
Date Modified: 2nd February 2023
File Folder: 6.1 - Inverse Functions + Derivates

```ad-abstract
title: Today's Topics
collapse: open

- Definition of Inverse Function
- Find Inverse Function of a One-to-One Function
- Relationshipo between graph of $f(x)$ and $f^-1(x)$

```

## Definition of Inverse Function

Let $f$ be a one to oen funciotn with a domain of $A$ and a range of $B$.

Its inverse function $f^-1(x)$ has a domain of $B$ and a range of $A$.

Is defined by:

$f^-1(y) = x$ ==if and only if== $f(x) = y$

```ad-info
title: Fact
- Domain of $f$ = Range of $f^-1$
- Range of $f$ = Domain of $f^-1$
```

```ad-info
title: Fact
color: 255, 127, 80

- $f^-1(f(x)) = x$ for all $x ∈ A$
- $f(f^-1(y)) = y$ for all $y ∈ B$
```


## Find Inverse of a One-to-One Function

### Step 1

Write $y = f(x)$

### Step 2

Solve this equation for $x$ in terms of $y$

### Step 3

To express $f^-1$ as a funciton of $x$.

*Interchange* $x$ and $y$.

The resulting equation is $y = f^-1(x)$

```ad-question
collapse: open
Find inverse fucntion of $f(x) = \frac{6-3x}{5x+7}$

```ad-check
title: Answer
collapse: open
-Step 1: $f(x)$ -> $y = \frac{6-3x}{5x+7}$
-Step 2: 
	- $y = \frac{6-3x}{5x+7}$
	- $y(5x + 7) = 6 - 3x$
	- $5xy + 7y = 6 - 3x$ 
	- $5xy + 3x = 6 - 7y$
		- Shift terms of x to one side and terms of y to the other side
	- $x(5y + 3) = 6 - 7y$
		- Take x out as a common factor
	- $x = \frac{6-7y}{5y+3}$
- Step 3:
	- $y = \frac{6-7x}{5x+3}$
- Solution: $f^-1(x) = 
```
```






