Date: 6th October 2023
Date Modified: 6th October 2023
File Folder: Week 7
#Physics1

```ad-abstract
title: Today's Topics
collapse: open

- Energy Cont

```

# Kinetic Energy Theorem

#comebacklater ex. 1

$$W_{net} = W_{N} + W_{mg} + W_{F} + W_{F_k}$$
$$W_{net} = F*d*\cos(0) - F_k*d*\cos(180) = (F-F_k)d$$

```ad-note
Remember Vector form:
$$F-F_k = ma$$
```

SO:
$$(F-F_k)d = m*a*d$$
```ad-note
Recall kinematic equations:
$$v^2=v_i^2+2a(x-x_i)$$
```

SO:

$$V_B^2 = V_A^2 = 2a*d$$
$$\frac{V^2_B-V^2_A}{2} = a*d$$

Replace $ad$ with solution of kinematic equation:

```ad-important
$$W_{net} = \frac{1}{2} mV_B^2 - \frac{1}{2} m V_A^2$$
$$W_{net} = kE_f - kE_i$$
$$W_{net} = \Delta kE$$
```

$$KE = \frac{1}{2}mV^2$$

# Potential Energy Theorem

## Gravitational

#comebacklater ex. 2

$$W_{mg} = mg * (h_A - h_B) \cos(0) = mgh_A - mgh_B$$
$$W_{mg} = U_i - U_f$$
$$W_{mg} = - \Delta U$$
```ad-warning
DO NOT FORGET THE NEGATIVE
```

```ad-note
title: Observations
- Gravitational Potential Energy is the energy of the object-Earth system
- Thus, the weight ($mg$) is an internal force of the system (object Earth)
- An internal force does work on the expense of the enrgy of the system $=> \space W_{mg} = - \Delta U$
```


```ad-important
Set the zero level of gravitational potential energy to the **lowest point** the object reaches in the problem to deal with the TRUE constant
$$U = mgh + L$$
```

### Applying the work - Kinetic Energy Theorem to EX. 2

$$W_{net} = W_{mg}$$
$$W_{mg} = \Delta KE = KE_B - KE_A$$
$$W_{mg} = KE_b - KE_A = U_A - U_B$$
$$Ke_B + U_B = KE_A+U_A$$
```ad-important
title: Conservation of Mechanical Energy
$$E_i = E_f$$

```ad-warning
This works **ONLY** in the absence of forces of friction
```

## Elastic

#comebacklater ex. 3

```ad-note
The force of elastic force changes as the displacement $x$ changes
```

$$W_{F_e} = \int_A^B F^{->}_e * dr^{->}$$
$$= \int_A^B (-kx)\hat{i} * (dx\hat{i} + dy\hat{j})$$
$$-k\int_A^Bxdx = -k\frac{1}{2}x^2 |^B_A = (-k\frac{1}{2}X_B^2) - (-k\frac{1}{2}X_A^2)$$
$$W_{F_e} = \frac{1}{2}kx_A^2 - \frac{1}{2} k_xB^2 = -\Delta U$$
THUS:

$$U = \frac{1}{2}kx^2$$


