Date: 4th February 2023
Date Modified: 4th February 2023
File Folder: 6.2 - Exponential Functions and Their Derivatives

```ad-abstract
title: Today's Topics
collapse: open

- Derivative/Integration of Natural Expoential Function
- Derivative/Integration of General Exponential Function
- Exponential Shifts
- Examples of Derivatives
- Examples of Integration

```

# Natural Exponential Function 

```ad-summary
title: Derivative
color: 242, 140, 40

$$\frac{d}{dx}(e^x) = e^xdx$$
```

The Derivative is the same as the exponential function because $f'(x) = f'(0)f(x)$

```ad-summary
title: Integration
color:

$$\int(e^xdx) = e^x + C$$
```

# General Exponential Function

```ad-summary
title: Derivative
color: 242, 140, 40

$$\frac{d}{dx}(a^x) = a^xln(a)$$
```


```ad-summary
title: Integration
color:

$$\int(a^xdx) = \frac{a^x}{ln(a)} + C$$
```


# Exponential Shifts

$f(x) = a^x + C$ will cause a vertical shift

$f(x) = a^{x+C}$ will cause a horizontal shift

# Examples with Derivatives


```ad-question
color: 0, 255, 255
Differentiate $y = e^{tanx}$

```ad-check
title: Solution
- Let $y=f(u) = e^u$, and $u(x) = tanx$ 
	- Utilize the chain rule
- $\frac{dy}{dx} = \frac{dy}{du} * \frac{du}{dx}
- $= e^u(sec^2x)$
- $= e^{tanx}(sec^2x)$
```



```ad-question
Differentiate $y = x^2e^{-3x}$
color: 0, 255, 255

```ad-check
title: Solution
- $\frac{d}{dx}*(x^2)e^{-3x} + x^2\frac{d}{dx}*(e^{-3x})$
	- Product Rule
- $2xe^{-3x} + x^2(e^{-3x}(-3))$
	- *note*: the $-3$ is the *dx* of *e^x*
- $y' = 2xe^{-3x} + -3x^2e^{-3x}$

```


```ad-question
color: 255, 255, 0
Differentiate $f(t) = tan(1 + e^{2t})$

```ad-check
title: Solution
- $f(u) = tanu$ and $u(t) = 1+e^{2t}$
	- Chain Rule Setup
- $sec^2(1+e^{2t})(2e^{2t})$
	- Differentiate (don't forget the $dt$)
- $y' = 2e^{2t}sec^2(1+e^{2t})$

```


# Examples of Integration


```ad-question

Differentiate $f(t) = tan(1 + e^{2t})$

```ad-check
title: Solution
- $f(u) = tanu$ and $u(t) = 1+e^{2t}$
	- Chain Rule Setup
- $sec^2(1+e^{2t})(2e^{2t})$
	- Differentiate (don't forget the $dt$)
- $y' = 2e^{2t}sec^2(1+e^{2t})$

```





 
 






