Date: 28th February 2023
Date Modified: 28th February 2023
File Folder: 6.7 - Hyberbolic Functions
#calculus2 

```ad-abstract
title: Today's Topics
collapse: open

- Defintions of Hyberbolic Functions
- Graphs of Hyberbolic Functions
- Hyberbolic Identities
- Derivatives of Hyberbolic Functions

```

# Definitions of Hyberbolic Functions

Hyberbolic Functions are derived from a combination of the natural exponenetial functions $e^x$ and $e^-x$ combined

1. $$sinh(x) = \frac{e^x-e^{-x}}{2}$$
2. $$cosh(x) = \frac{e^x+e^{-x}}{2}$$
3. $$csch(x) = \frac{2}{e^x-e^{-x}}$$
4. $$sech(x)=\frac{2}{e^x+e^{-x}}$$
5. $$tanh(x) = \frac{e^x-e^{-x}}{e^x+e^{-x}}$$
6. $$coth(x) = \frac{e^x+e^{-x}}{e^x-e^{-x}}$$
# Hyberbolic Function Identities

1. $$sinh(-x) = -sinh(x)$$
2. $$cosh(-x)=cosh(x)$$                                                                               ==Because cosh(x) is always positive and even
3. $$cosh^2(x) - sinh^2(x) = 1$$                                                                              ==Same trig Identity but with a negatvie sign instead
4. $$sech^2(x)=1-tanh^2(x)$$
5. $$sinh(x+y)=sinh(x)cosh(y)+cosh(x)sinh(y)$$
6. $$cosh(x+y)=cosh(x)cosh(y) + sinh(x)sinh(y)$$                                                     ==Same as trig identity but the second term is positive instead of negative


```ad-note
Identities often only have one variable AND are true for all values of that variable
```

# Derivatives of Hyberbolic Functions

1. $$\frac{d}{dx}(sinh(x))=cosh(x)$$
2. $$\frac{d}{dx}(cosh(x)) = sinh(x)$$
3. $$\frac{d}{dx}(tanh(x)) = sech^2(x)$$
4. $$\frac{d}{dx}(csch(x)) = -csch(x)coth(x)$$
5. $$\frac{d}{dx}(sech(x)=-sech(x)tanh(x)$$
6. $$\frac{d}{dx}(coth(x)) = -csch^2(x)$$
```ad-important
These Derivatives are the same as the standard trig functions, **except** for **two** of them:
- $cosh(x)$ becomes **positive** $sinh(x)$
- $sech(x)$ becomes **negative** $sech(x)tanh(x)$
```

```ad-question
### If $y = cosh(sqrt{x})$, find $\frac{dy}{dx}$

```ad-check
title: Solution
- #### $\frac{dy}{dx} = sinh(\sqrt{x})(\frac{1}{2\sqrt{x}})$
	- use $\frac{d}{dx}(cosh(x)) = sinh(x)$ plus chain rule the inner function to find the derivative
- #### $\frac{dy}{dx} = \frac{sinh(\sqrt{x})}{2\sqrt{x}}$
	- Simplify to get final answer
```



