Date: 3rd March 2023
Date Modified: 3rd March 2023
File Folder: 6.7 - Hyberbolic Functions
#calculus2 

```ad-abstract
title: Today's Topics
collapse: open

- Inverse Hyperbolic Definitions
- Inverse Hyberbolic Functions
- Derivatives of Inverse Hyberbolic Functions
- Examples of:
	- Derivatives
	- Limits
	- Integration

```

# Inverse Hyberbolic Defintions

1. $y=sinh^-1(x)$ when $sinh(y)=x$
2. $y=cosh^-1(x)$ when $cosh(y)=x$ **AND** $[0, \infty$]
3. $y=tanh^-1(x)$ when $tanh(y)=x$

# Inverse Hyperbolic Functions

1. $sinh^-1(x) = \ln(x+\sqrt{x^2+1})$ for $(-\infty, \infty)$
2. $cosh^-1(x) = \ln(x + \sqrt{x^2-1})$ for $[1, \infty)$
3. $tanh^-1(x) = \frac{1}{2}\ln(\frac{1+x}{1-x}))$ for $(-1, 1)$

```ad-important
To remember what these inverses equal, remember that Hyperbolic Functions are derived from natural exponential functions, and the inverse of natural exponential functions is always natural logarithms.
```


# Derivatives of Inverse Hyperbolic Functions

1. $$\frac{d}{dx}sinh^-1(x) = \frac{1}{\sqrt{1+x^2}}$$
2. $$\frac{d}{dx} cosh^-1(x) = \frac{1}{\sqrt{x^2-1}}$$
3. $$\frac{d}{dx}tanh^-1(x)=\frac{1}{1-x^2}$$
4. $$\frac{d}{dx}csch^-1(x) = \frac{-1}{|x| \sqrt{x^2+1}}$$
5. $$\frac{d}{dx}sech^-1(x) = \frac{-1}{x \sqrt{1-x^2}}$$
6. $$\frac{d}{dx}coth^-1(x)=\frac{1}{1-x^2}$$
```ad-note
Title: Differences between Inverse Trigonometric and Inverse Hyperbolic Functions
- $sin^-1(x)$ and $sinh^-1(x)$ are the same, but the inner function is **Positive**
	- $1-x^2$ vs. $1+x^2$
- $sinh^-1(x)$ and $cosh^-1(x)$ are the same, but the constant 1 becomes **Negative**
	- $1+x^2$ vs $x^2-1$
- $csc^-1(x)$ and $csch^-1(x)$ are the same, but the inner fucniton is **Positive** AND the leading coefficent gets taken to its ==absolute value==
	- $x\sqrt{x^2-1}$ vs $|x|\sqrt{x^2+1}$
- $tan^-1(x)$ and $tanh^-1(x)$ are the same, but the $x^2$ term is **Negative**
	- $1+x^2$ vs $1-x^2$
- $coth^-1(x)$ and $tanh^-1(x)$ **are the same**
```


# Inverse Hyperbolic Examples

## Derivatives

## Limits

## Integration