Date: 14th March 2023
Date Modified: 14th March 2023
File Folder: 6.8 - Indeterminate Forms and L' Hospital's Rule
#calculus2 #year1 #semester2

```ad-abstract
title: Today's Topics
collapse: open

- L' Hospital Rule Definition
- Examples
```

# L' Hospital Rule Defintion

```ad-note
L' Hospital Rule is the most powerful tool for solving the indeterminate forms with limits
```

Suppose that $f$ and $g$, are differentiable and $g(x) \ne 0$ on an open interval $I$ that contians $a$ except possibly at $a$

**For the following situations:
- $\lim_{x \to a} f(x) = 0$, and $lim_{x \to a} g(x) = 0$ 
	- $\frac{0}{0}$ indeterminate form
- $\lim_{x \to a} f(x) = \pm \infty$ and $\lim_{x \to a} g(x) = \pm \infty$

Then: $$lim_{x \to a} = \frac{f(x)}{g(x)} = lim_{x \to a} = \frac{f'(x)}{g'(x)}$$
# Examples

## $\frac{0}{0}$ form

```ad-question
#### Find $lim_{x \to 1} \frac{x^7 - 1}{x^3 - 1}$

```ad-check
title: solution
- $\frac{(1)^7-1}{(1)^3-1} = \frac{0}{0}$ form
	- When replacing $x$ with $1$ to solve the limit, the limit becomes indeterminate, thus...
-  $lim_{x \to 1} \frac{\frac{d}{dx}(x^7 - 1)}{\frac{d}{dx}(x^3 - 1)} = lim_{x \to 1} \frac{7x^6}{3x^2}$
	- Use L' Hospital Rule to find its true limit
- $\frac{7(1)^6}{3(1)^2}$ 
	- Replace $x$ with $1$ to solve the limit
- $\frac{7}{3}$
	- Simplify to find final answer
```

## $\frac{\infty}{\infty}$ form

```ad-question
#### Calculate $\lim_{x \to \infty} \frac{e^x}{x^2}$

```ad-check
title: solution
- $\frac{e^{(\infty)}}{(\infty)^2} = \frac{\infty}{\infty}$ Form
	- Replace $x$ by $\infty$ to find the limit. Because it is in \frac{\infty}{\infty}$ Form, utilize L' Hospital Rule
- $\lim_{x \to \infty} \frac{e^x}{2x} = \frac{e^{(\infty)}}{2(\infty)} = \frac{/infty}{/infty}$
	- Take the derivative of the top and the bottom. When the limit is found, you can see that it still is in indeterminate form.
	- **Thus, L' Hospitals Rule can be taken again.**
- $lim_{x \to \infty} \frac{e^x}{2} = \frac{e^{(\infty)}}{2} = \infty$
	- Once L' Hopsitals Rule is taken for a 2nd time, the limit can be solved
```

## $\infty - \infty$ Form

```ad-important
You can take the limit of $\infty - \infty$ form using L' Hospital's Rule by converting it to either $\frac{0}{0}$ or $\frac{\infty}{\infty}$ form
```


```ad-question
#### Find $\lim_{x \to 0^+} (\frac{1}{x} - \frac{1}{e^x-1})$
```ad-check
- $\frac{1}{(0)} - \frac{1}{(0)} = \infty - \infty$
	- When the limit is taken from the equation, it is found to be in $\infty - \infty$ form thus...
- $\lim_{x \to 0^+} \frac{e^x-1-x }{x(e^x-1)}$
	- Combine the fractions
- $\frac{e^{(0)}-1-(0)}{(0)(e^{(0)}-1)} = \frac{0}{0} form$
	- By combining the fractions, you are able to solve for the limit into an indeterminate form
- $\lim_{x \to 0^+} \frac{e^x-1}{xe^x+e^x-1}$
	- Use L' Hospital's Rule and take the first derivative of the top and bottom
- $\frac{e^{(0)}-1}{(0)e^{(0)}+e^{(0)}-1} = \frac{0}{0}$
	- Take the limit and find that it is still in $\frac{0}{0}$ form, so...
- $\lim_{x \to 0^+} \frac{e^x}{xe^x+2e^x}$
	- Take the derivative of the top and bottom once again.
- $\frac{e^{(0)}}{(0)e^{(0)}+2e^{(0)}} = \frac{1}{2}$
	- Take the limit by replacing $x$ by $0$ on the right side. It is found that the limit is actually $\frac{1}{2}$
```

## $0 * \infty$ form

```ad-note
Same as the previous. Make sure it is in the proper forms
```

```ad-question
#### Evaluate $\lim_{x \to 0} xln(x)$

```ad-check
title: Solution
- $(0)ln(0) = 0 * \infty form$
	- When the limit is taken, it gets in a form that cannot be used by L' Hospital's Rule, so...
- $\lim_{x \to 0} \frac{ln(x)}{\frac{1}{x}} = \frac{\infty}{\infty} form$
	- By putting the $x$ to the bottom as \frac{1}{x} in the denominator to make it as an $/frac{\infty}{\infty}$ form so...
- $\lim_{x \to 0} \frac{\frac{1}{x}}{\frac{-1}{x^2}} = \lim_{x \to 0} -x$
	- Taking the first derivative of both the top and the bottom, the limit is able to be reduced significantly
- $\lim_{x \to 0} -x = 0$
	- Replacing $x$ by 0 will give us the final limit
```





